---
keywords: fastai
description: Calculus summary note.
title: "[Calculus] CH03. Taylor Expansion"
toc: false
badges: false
comments: false
categories: [calculus]
hide_{github,colab,binder,deepnote}_badge: true
nb_path: _notebooks/ch03-taylor-expansion.ipynb
layout: notebook
---

<!--
#################################################
### THIS FILE WAS AUTOGENERATED! DO NOT EDIT! ###
#################################################
# file to edit: _notebooks/ch03-taylor-expansion.ipynb
-->

<div class="container" id="notebook-container">
        
<div class="cell border-box-sizing text_cell rendered"><div class="inner_cell">
<div class="text_cell_render border-box-sizing rendered_html">
<h4 id="3.1.-Mutivariate-Taylor-Polynomial">3.1. Mutivariate Taylor Polynomial<a class="anchor-link" href="#3.1.-Mutivariate-Taylor-Polynomial"> </a></h4><h5 id="Definition.3.1.-First-Order-Taylor-Polynomial(Linear-Approximation)">Definition.3.1. First Order Taylor Polynomial(Linear Approximation)<a class="anchor-link" href="#Definition.3.1.-First-Order-Taylor-Polynomial(Linear-Approximation)"> </a></h5><p>Let $f: \mathbb{R}^n \rightarrow \mathbb{R}$ be a differentiable function.<br>
Then first order taylor polynomial of $f$ at $\mathbf{x}_0$ is</p>
$$
P_1(\mathbf{\mathbf{x}}) = f(\mathbf{x}_0) + (\mathbf{x} - \mathbf{x}_0)^T \nabla_\mathbf{x} f(\mathbf{x}_0).
$$
</div>
</div>
</div>
<div class="cell border-box-sizing text_cell rendered"><div class="inner_cell">
<div class="text_cell_render border-box-sizing rendered_html">
<h5 id="Definition.3.2.-Second-Order-Taylor-Polynomial">Definition.3.2. Second Order Taylor Polynomial<a class="anchor-link" href="#Definition.3.2.-Second-Order-Taylor-Polynomial"> </a></h5><p>Let $f: \mathbb{R}^n \rightarrow \mathbb{R}$ be a twice differentiable function.<br>
Then second order taylor polynomial of $f$ at $\mathbf{x}_0$ is</p>
$$
P_2(\mathbf{\mathbf{x}}) = f(\mathbf{x}_0) + (\mathbf{x} - \mathbf{x}_0)^T \nabla_\mathbf{x} f(\mathbf{x}_0) + \frac{1}{2!} (\mathbf{x} - \mathbf{x}_0)^T \nabla_\mathbf{x}^2 f(\mathbf{x}_0) (\mathbf{x} - \mathbf{x}_0)
$$
</div>
</div>
</div>
<div class="cell border-box-sizing text_cell rendered"><div class="inner_cell">
<div class="text_cell_render border-box-sizing rendered_html">
<p>We don't need more than this.</p>

</div>
</div>
</div>
</div>
 

